current/colorConvStack.v
@@ -1,36 +1,188 @@
-Require Import ThreeSatReduction. 
+Require Import ThreeSatReduction.   
 
-Theorem convFormulaColorable : forall i Gamma Delta G F eta U S1 S2 S3 S4 S5 eta' C, 
-                                 valid Gamma C F eta' eta -> 
-                                 uniqueLockstep S1 S2 S3 S4 Gamma ->
+
+
+
+Theorem convertBaseColorable : forall i Gamma Delta G F eta S5 eta'' eta' C, 
+                                 setVertices Gamma C 0 eta' eta -> 
+                                 setCs eta' (3 * length Gamma) F eta'' eta -> 
                                  genericUnique S5 (fun x => x) Delta -> 
-                                 genericUnique U (fun a=>match a with (x,y) => x end) eta' ->
-                                 convFormula i Gamma Delta F G -> coloring eta' G C.
-Proof. 
-  intros. inv H3. simpl. destruct e1. destruct e2. destruct e3. 
-  
-Theorem convertBaseColorable : forall i Gamma Delta G F eta U S1 S2 S3 S4 S5 eta' C, 
-                                 valid Gamma C 1 eta' eta -> 
-                                 uniqueLockstep S1 S2 S3 S4 Gamma ->
-                                 genericUnique S5 (fun x => x) Delta -> 
-                                 genericUnique U (fun a=>match a with (x,y) => x end) eta' ->
                                  convert_base Gamma Delta i G -> coloring eta' G C.
+Admitted. 
 
-
-
-
-
-
-Theorem convStackColorable : forall i Gamma Delta K G eta U S1 S2 S3 S4 S5 eta' C, 
-                               valid Gamma C 1 eta' eta -> 
-                               uniqueLockstep S1 S2 S3 S4 Gamma ->
-                               genericUnique S5 (fun x => x) Delta -> 
-                               genericUnique U (fun a=>match a with (x,y) => x end) eta' ->
-                               convStack i Gamma Delta K G -> coloring eta' G C.
+Theorem colorWeakeningApp : forall eta1 eta2 eta3 G C,
+                           coloring (eta1++eta3) G C ->
+                           coloring (eta1++eta2++eta3) G C. 
 Proof.
-  intros. genDeps {{ U; S1; S2; S3; S4; S5; eta; eta'; C }}. induction H3; intros. 
+  intros. genDeps {{ eta2 }}. remember(eta1++eta3). induction H; intros. 
   {constructor. }
-  {constructor. eapply IHconvStack; eauto. eapply convFormulaColorable; eauto. }
+  {subst. econstructor. apply in_app_iff in H. inv H. auto. apply in_app_iff; simpl.
+   eauto. repeat rewrite in_app_iff. auto. apply in_app_iff in H0. inv H0; 
+   repeat rewrite in_app_iff; eauto. auto. auto. auto. eapply IHcoloring; eauto. }
+  {constructor; eauto. }
 Qed. 
 
+Theorem consApp : forall (A:Type) (hd:A) tl, hd::tl = [hd]++tl. auto. Qed. 
+Theorem plus0 : forall n, n = n + 0. auto. Qed. 
+
+Ltac negate H :=
+  match type of H with
+      |?x => assert(~ x)
+  end. 
+
+Theorem InEtaInEta' : forall u c b Gamma C i eta eta', In (u, b) eta -> In (3*u, c) eta' -> 
+                                            setVertices Gamma C i eta' eta -> 
+                                            (c = u /\ In (u, true) eta) \/ (c = C /\ In (u, false) eta). 
+Proof.
+  intros. genDeps {{ u; c; b }}. induction H1; intros. 
+  {destruct (eq_nat_dec u u0). 
+   {subst. inCons. invertTupEq. left. split; simpl; auto. inCons. invertTupEq. omega. 
+    inCons. invertTupEq. omega. negate H3. assert(3*u0=3*u0+0) by auto. rewrite H2. 
+    eapply notInEta; eauto. contradiction. }
+   {inCons. invertTupEq. omega. inCons. invertTupEq. omega. inCons. invertTupEq. 
+    omega. inCons. invertTupEq. omega. eapply IHsetVertices in H3; eauto. inv H3. invertHyp. 
+    left. split; simpl; auto. invertHyp. right. split; simpl; auto. }
+  }
+  {destruct (eq_nat_dec u u0). 
+   {subst. inCons. invertTupEq. right. split; simpl; auto. inCons. invertTupEq. omega. 
+    inCons. invertTupEq. omega. negate H3. assert(3*u0=3*u0+0) by auto. rewrite H2. 
+    eapply notInEta; eauto. contradiction. }
+   {inCons. invertTupEq. omega. inCons. invertTupEq. omega. inCons. invertTupEq. 
+    omega. inCons. invertTupEq. omega. eapply IHsetVertices in H3; eauto. inv H3. invertHyp. 
+    left. split; simpl; auto. invertHyp. right. split; simpl; auto. }
+  }
+  {inv H. }
+Qed. 
+
+
+Theorem lookupEta'Det : forall Gamma C i eta eta' epsilon u c1 c2, setVertices Gamma C i eta' eta ->
+                                         In (3*u+epsilon, c1) eta' -> In (3*u+epsilon, c2) eta' -> c1=c2 . 
+Proof.
+  intros. induction H. 
+  {destruct (eq_nat_dec u u0). 
+   {subst. inCons. invertTupEq. inCons. invertTupEq. auto. inCons. 
+    invertTupEq. omega. inCons. invertTupEq. auto. negate H1. eapply notInEta; eauto. 
+    destruct epsilon. auto. omega. contradiction. inCons. invertTupEq. inCons. invertTupEq. 
+    omega. inCons. invertTupEq. auto. inCons. invertTupEq. omega. negate H1.
+    eapply notInEta; eauto. destruct epsilon. auto. omega. contradiction. inCons. invertTupEq. 
+    inCons. invertTupEq. auto. inCons. invertTupEq. omega. inCons. invertTupEq. auto.
+    negate H1. eapply notInEta; eauto. destruct epsilon. auto. omega. contradiction. inCons. 
+    invertTupEq. negate H3. eapply notInEta; eauto. destruct epsilon. auto. omega. contradiction. 
+    inCons. invertTupEq. negate H3. eapply notInEta; eauto. destruct epsilon. auto. omega. 
+    contradiction. inCons. invertTupEq. negate H3. eapply notInEta; eauto. destruct epsilon. 
+    auto. omega. contradiction. eapply IHsetVertices; eauto. }
+   {subst. inCons. invertTupEq. destruct epsilon. omega. destruct epsilon. omega. 
+
+invertTupEq. inCons. invertTupEq. auto. inCons. 
+    invertTupEq. omega. inCons. invertTupEq. auto. negate H1. eapply notInEta; eauto. 
+    omega. destruct epsilon. auto. omega. contradiction. inCons. invertTupEq. inCons. invertTupEq. 
+    omega. inCons. invertTupEq. auto. inCons. invertTupEq. omega. negate H1.
+    eapply notInEta; eauto. destruct epsilon. auto. omega. contradiction. inCons. invertTupEq. 
+    inCons. invertTupEq. auto. inCons. invertTupEq. omega. inCons. invertTupEq. auto.
+    negate H1. eapply notInEta; eauto. destruct epsilon. auto. omega. contradiction. inCons. 
+    invertTupEq. negate H3. eapply notInEta; eauto. destruct epsilon. auto. omega. contradiction. 
+    inCons. invertTupEq. negate H3. eapply notInEta; eauto. destruct epsilon. auto. omega. 
+    contradiction. inCons. invertTupEq. negate H3. eapply notInEta; eauto. destruct epsilon. 
+    auto. omega. contradiction. eapply IHsetVertices; eauto. }
+
+
+Theorem helper : forall Gamma C p1 eta eta' i c G u eta'' v v0 u', 
+              u = getVar p1 -> setVertices Gamma C 0 eta' eta -> In (u,3*u,3*u+1,3*u+2) Gamma -> winner eta p1 u' ->
+              mkEdge i p1 (3*u) (3*u+1) (v,v0) -> In (3 * u', c) eta' -> 
+              coloring(eta' ++ (i,c)::eta'') G C ->
+              coloring(eta' ++ (i,c)::eta'') (newEdge v v0 G) C.
+Proof.
+  intros. inversion H3; subst. 
+  {inv H2. 
+   {copy H1. eapply V_V'MapToUOrC in H1; eauto. inv H1. 
+    {invertHyp. eapply InEtaInEta' in H6; eauto. simpl in *. inv H6. 
+     {admit. }
+     {invertHyp. econstructor. apply in_app_iff. right. simpl. eauto. apply in_app_iff. 
+      left. eauto. auto. omega. omega. omega.  auto. }
+    }
+    {invertHyp. econstructor. apply in_app_iff. right. simpl. eauto. apply in_app_iff. 
+     left. eauto. 
+
+Theorem convFormulaColorable : forall i Gamma Delta G eta K U eta'' F eta' C, 
+                                 setVertices Gamma C 0 eta' eta -> SAT' eta (F::K) ->
+                                 setCs eta' i (F::K) eta'' eta -> 
+                                 genericUnique U (fun x => x) Delta -> 
+                                 convFormula i Gamma Delta F G -> coloring (eta'++eta'') G C.
+Proof. 
+  intros. inv H3. simpl. destruct e1. destruct e2. destruct e3.
+  {inv H1.  
+   {inversion H8; subst. simpl in *. 
+    {inv H18.  
+     {copy H4. eapply V_V'MapToUOrC in H4; eauto. inv H4. 
+      {invertHyp. inv H0. econstructor. apply in_app_iff. simpl. right. eauto. 
+       apply in_app_iff. left. eauto. 
+
+
+
+ copy H3. eapply InEtaInEta' in H3; eauto. inv H3. 
+       {invertHyp. econstructor. apply in_app_iff. right. simpl. eauto. apply in_app_iff. 
+        left. eauto. 
+
+Focus 2. 
+       invertHyp. econstructor. apply in_app_iff. right. simpl. eauto. apply in_app_iff.
+       left. eauto. auto. omega. omega. omega. 
+
+
+
+Theorem A : forall Gamma u C eta eta', 
+              setVertices Gamma C 0 eta' eta -> In (u,3*u,3*u+1,3*u+2) Gamma ->
+              coloring
+
+Theorem convStackColorable : forall i Gamma Delta G eta F j S5 eta'' eta' C, 
+                               setVertices Gamma C 0 eta' eta -> 
+                               setCs eta' j F eta'' eta ->
+                               genericUnique S5 (fun x => x) Delta -> 
+                               convStack i Gamma Delta F G -> coloring (eta' ++ eta'') G C.
+Proof.
+  intros. genDeps {{ S5; eta; eta'; C; eta''; j }}. induction H2; intros. 
+  {constructor. }
+  {constructor. 
+   {inv H1. 
+    {rewrite consApp. apply colorWeakeningApp. eapply IHconvStack; eauto. }
+    {rewrite consApp. apply colorWeakeningApp. eapply IHconvStack; eauto. }
+    {rewrite consApp. apply colorWeakeningApp. eapply IHconvStack; eauto. }
+   }
+   {eapply convFormulaColorable; eauto. }
+  }
+Qed. 
+
+
+
+
+
+
+  
+
+
+
+
+
+
+
+
+
+
+
+
+
+
+
+
+
+
+
+
+
+
+
+
+
+
+
+ad;lfkhjasdf
 
