current/colorVarsToClique.v
@@ -1,90 +1,5 @@
 Require Export ThreeSatReduction. 
 
-
-Theorem XMapsToU : forall u Gamma C eta' eta i, 
-                     In (u,3*u,3*u+1,3*u+2) Gamma -> 
-                     setVertices Gamma C i eta' eta -> In (3*u+2,u) eta' /\ u < C.
-Proof. 
-  intros. induction H0. 
-  {destruct (eq_nat_dec u u0). 
-   {inCons. invertTupEq. simpl. split; auto. split. simpl. auto. omega. }
-   {inCons. invertTupEq. omega. eapply IHsetVertices in H2; eauto. invertHyp. 
-    split. simpl. auto. auto. }
-  }
-  {destruct (eq_nat_dec u u0). 
-   {inCons. invertTupEq. simpl. split; auto. split. simpl. auto. omega. }
-   {inCons. invertTupEq. omega. eapply IHsetVertices in H2; eauto. invertHyp. 
-    split. simpl. auto. auto. }
-  }
-  {inv H. }
-Qed. 
-
-Theorem V_V'MapToUOrC : forall u Gamma C eta' eta i, 
-                          In (u,3*u,3*u+1,3*u+2) Gamma -> 
-                          setVertices Gamma C i eta' eta -> 
-                          (In (3*u,u) eta' /\ u < C /\ In (3*u+1,C) eta') \/
-                          (In (3*u,C) eta' /\ u < C /\ In (3*u+1,u) eta').
-Proof.
-  intros. induction H0. 
-  {destruct (eq_nat_dec u u0). 
-   {subst. inCons. invertTupEq. left. simpl. auto. eapply IHsetVertices in H2. inv H2. 
-    invertHyp. left. simpl. auto. invertHyp. left. simpl. auto. }
-   {inCons. invertTupEq. omega. eapply IHsetVertices in H2. inv H2. invertHyp.
-    left. split. simpl. auto. split. auto. simpl. auto. invertHyp. right. 
-    simpl. split; auto. }
-  }
-  {destruct (eq_nat_dec u u0). 
-   {subst. inCons. invertTupEq. right. simpl. auto. eapply IHsetVertices in H2. inv H2. 
-    invertHyp. right. simpl. auto. invertHyp. right. simpl. auto. }
-   {inCons. invertTupEq. omega. eapply IHsetVertices in H2. inv H2. invertHyp.
-    left. split. simpl. auto. split. auto. simpl. auto. invertHyp. right. 
-    simpl. split; auto. }
-  }
-  {inv H. }
-Qed. 
-
-Theorem edgesNeq : forall Gamma C eta' eta u i u0,
-                     In (u,3*u,3*u+1,3*u+2) Gamma -> In (u0,3*u0,3*u0+1,3*u0+2) Gamma ->
-                     setVertices Gamma C i eta' eta -> u <> u0 ->
-                     exists c1 c2, In (3*u, c1) eta' /\ In (3*u0+2, c2) eta' /\
-                              c1 <= C /\ c2 <= C /\ c1 <> c2. 
-Proof.
-  intros. genDeps {{ u; u0 }}. induction H1; intros. 
-  {inCons. 
-   {inCons. 
-    {invertTupEq. omega. }
-    {invertTupEq. exists u1. copy H1. eapply InSetVertices in H1; eauto. invertHyp. 
-     exists x. split. simpl. auto. split. simpl. auto. split; auto. omega. split; auto. 
-     eapply geSetVertices in H0; eauto. omega. }
-   }
-   {inCons. 
-    {invertTupEq. eapply V_V'MapToUOrC in H4; eauto. inv H4; invertHyp.  
-     {exists u1. exists u0. split; simpl; auto. split; auto. split. omega. split; auto. omega. }
-     {exists C. exists u0. split. simpl. auto. split. simpl. auto. split; auto. split; omega. }
-    }
-    {eapply IHsetVertices in H4; eauto. invertHyp. exists x. exists x0. split. simpl. auto. 
-     split. simpl. auto. split; auto. }
-   }
-  }
-  {inCons. 
-   {inCons. 
-    {invertTupEq. omega. }
-    {invertTupEq. exists C. copy H1. eapply XMapsToU in H1; eauto. invertHyp. exists u0. split. 
-     simpl. auto. split. simpl. auto. split; auto. split; omega. }
-   }
-   {inCons. 
-    {invertTupEq. eapply V_V'MapToUOrC in H4; eauto. inv H4. 
-     {invertHyp. exists u1. exists u0. split. simpl. auto. split. simpl. auto. split; auto. 
-      omega. split; auto. omega. }
-     {invertHyp. exists C. exists u0. split. simpl. auto. split. simpl. auto. split; auto. split; omega. }
-    }
-    {eapply IHsetVertices in H4; eauto. invertHyp. exists x. exists x0. split. simpl. auto. 
-     split. simpl. auto. split; auto. }
-   }
-  }
-  {inv H. }
-Qed. 
-
 Theorem connectXColorable : forall Gamma Delta G C eta eta' u, 
                               ~In u Delta -> setVertices Gamma C 0 eta' eta -> In (u,3*u,3*u+1,3*u+2) Gamma ->
                               connectX Gamma Delta (3*u) G -> coloring eta' G C. 
@@ -93,13 +8,48 @@ Proof.
   {constructor. } 
   {subst. destruct(eq_nat_dec u u0). 
    {subst. exfalso. apply H. simpl. auto. }
-   {copy H3. eapply edgesNeq in H3. Focus 2. eauto. Focus 2. eapply H0. invertHyp. 
-    econstructor; eauto. eapply IHconnectX; eauto. intros c. apply H. simpl. auto.
-    eauto. }
+   {copy H3. copy H1. eapply V_V'MapToUOrC in H1; eauto. eapply XMapsToU in H0; eauto. 
+    inv H1. invertHyp. econstructor; eauto. omega. omega. eapply IHconnectX; eauto. 
+    intros c. apply H. simpl; auto. invertHyp. econstructor; eauto. omega. 
+    omega. eapply IHconnectX; eauto. intros c. apply H. simpl; auto. }
   }
 Qed. 
 
-Theorem cliqueColorable : forall Gamma eta Delta C G eta' S5, 
+Theorem connectXColorable' : forall Gamma Delta G C eta eta' u, 
+                              ~In u Delta -> setVertices Gamma C 0 eta' eta -> In (u,3*u,3*u+1,3*u+2) Gamma ->
+                              connectX Gamma Delta (3*u+1) G -> coloring eta' G C. 
+Proof.
+  intros. genDeps {{ eta; C; eta'}}. remember (3*u+1). induction H2; intros. 
+  {constructor. } 
+  {subst. destruct(eq_nat_dec u u0). 
+   {subst. exfalso. apply H. simpl. auto. }
+   {copy H3. copy H1. eapply V_V'MapToUOrC in H1; eauto. eapply XMapsToU in H0; eauto. 
+    inv H1. invertHyp. econstructor; eauto. omega. omega. eapply IHconnectX; eauto. 
+    intros c. apply H. simpl; auto. invertHyp. econstructor; eauto. omega. 
+    omega. eapply IHconnectX; eauto. intros c. apply H. simpl; auto. }
+  }
+Qed. 
+
+
+Theorem connectVColorable : forall Gamma Delta G C eta eta' u, 
+                              ~In u Delta -> setVertices Gamma C 0 eta' eta -> In (u,3*u,3*u+1,3*u+2) Gamma ->
+                              connectV Gamma Delta (3*u+2) G -> coloring eta' G C. 
+Proof.
+  intros. genDeps {{ eta; C; eta'}}. remember (3*u+2). induction H2; intros. 
+  {constructor. } 
+  {subst. destruct(eq_nat_dec u u0). 
+   {subst. exfalso. apply H. simpl. auto. }
+   {copy H3. copy H1. eapply XMapsToU in H1; eauto. eapply V_V'MapToUOrC in H0; eauto. 
+    inv H0. 
+    {invertHyp. econstructor; eauto; try omega. econstructor; eauto; try omega. 
+     eapply IHconnectV; eauto. intros contra. apply H. simpl. auto. }
+    {invertHyp. econstructor; eauto; try omega. econstructor; eauto; try omega. 
+     eapply IHconnectV; eauto. intros contra. apply H. simpl; auto. }
+   }
+  }
+Qed. 
+
+Theorem varsToCliqueColorable : forall Gamma eta Delta C G eta' S5, 
                             setVertices Gamma C 0 eta' eta -> 
                             genericUnique S5 (fun x => x) Delta -> 
                             vars_to_clique Gamma Delta G -> coloring eta' G C. 
@@ -108,10 +58,10 @@ Proof.
   {constructor. }
   {constructor. eapply IHvars_to_clique; eauto. inv H5. eauto. constructor. 
    eapply connectXColorable; eauto. eapply genericUniqueNotIn; eauto. Focus 2. inv H5. 
-   eauto. apply Union_intror. constructor. 
+   eauto. apply Union_intror. constructor. constructor. eapply connectXColorable'; eauto. 
+   inv H5. eapply genericUniqueNotIn. Focus 2. eauto. apply Union_intror. constructor. 
+   eapply connectVColorable; eauto. inv H5. eapply genericUniqueNotIn. Focus 2. eauto. 
+   apply Union_intror. constructor. }
+Qed. 
 
 
-
-
-
-asdfasdfsadf
